Generalize tlet reduction induction

CoreLang/theories/Sugar.v
@@ -17,8 +17,12 @@ Definition tbool_gen : tm :=
 Definition tnat_gen : tm :=
   tprim op_nat_gen vtrue.
 
-Definition tapp_tm (ef : tm) (vx : value) : tm :=
-  tlete ef (tapp (vbvar 0) vx).
+Fixpoint tapp_tm (ef : tm) (vx : value) : tm :=
+  match ef with
+  | tret vf => tapp vf vx
+  | tlete e1 e2 => tlete e1 (tapp_tm e2 vx)
+  | _ => tlete ef (tapp (vbvar 0) vx)
+  end.
 
 Definition tchoice (etrue efalse : tm) : tm :=
   tlete tbool_gen (tmatch (vbvar 0) etrue efalse).
@@ -32,7 +36,21 @@ Proof. repeat constructor. Qed.
 Lemma fv_tapp_tm ef vx :
   fv_tm (tapp_tm ef vx) = fv_tm ef ∪ fv_value vx.
 Proof.
-  unfold tapp_tm. simpl. set_solver.
+  induction ef; simpl; set_solver.
+Qed.
+
+Lemma open_tapp_tm_lc_arg ef vx k u :
+  lc_value vx →
+  open_tm k u (tapp_tm ef vx) = tapp_tm (open_tm k u ef) vx.
+Proof.
+  intros Hvx. revert k.
+  induction ef; intros k; simpl;
+    try rewrite (open_rec_lc_value vx Hvx k u);
+    try rewrite (open_rec_lc_value vx Hvx (S k) u);
+    try (destruct (decide (S k = 0)); [lia | reflexivity]);
+    try reflexivity.
+  rewrite IHef2.
+  reflexivity.
 Qed.
 
 Lemma body_tapp_tm_body vx :
@@ -50,12 +68,28 @@ Lemma lc_tapp_tm ef vx :
   lc_value vx →
   lc_tm (tapp_tm ef vx).
 Proof.
-  intros Hef Hvx. unfold tapp_tm.
-  eapply LC_lete with (L := ∅); [exact Hef |].
-  intros x _.
-  change (lc_tm (tapp (vfvar x) (open_value 0 (vfvar x) vx))).
-  rewrite (open_rec_lc_value vx Hvx 0 (vfvar x)).
-  repeat constructor. exact Hvx.
+  intros Hef. revert vx.
+  induction Hef; intros vx Hvx; simpl.
+  - repeat constructor; eauto.
+  - eapply LC_lete; [exact Hef |].
+    intros x Hx.
+    rewrite open_tapp_tm_lc_arg by exact Hvx.
+    eauto.
+  - eapply LC_lete with (L := ∅); [constructor; exact H |].
+    intros x _.
+    change (lc_tm (tapp (vfvar x) (open_value 0 (vfvar x) vx))).
+    rewrite (open_rec_lc_value vx Hvx 0 (vfvar x)).
+    repeat constructor. exact Hvx.
+  - eapply LC_lete with (L := ∅); [constructor; assumption |].
+    intros x _.
+    change (lc_tm (tapp (vfvar x) (open_value 0 (vfvar x) vx))).
+    rewrite (open_rec_lc_value vx Hvx 0 (vfvar x)).
+    repeat constructor. exact Hvx.
+  - eapply LC_lete with (L := ∅); [constructor; assumption |].
+    intros x _.
+    change (lc_tm (tapp (vfvar x) (open_value 0 (vfvar x) vx))).
+    rewrite (open_rec_lc_value vx Hvx 0 (vfvar x)).
+    repeat constructor. exact Hvx.
 Qed.
 
 Lemma basic_typing_tapp_tm Γ ef vx Tx T :
@@ -63,33 +97,38 @@ Lemma basic_typing_tapp_tm Γ ef vx Tx T :
   Γ ⊢ᵥ vx ⋮ Tx →
   Γ ⊢ₑ tapp_tm ef vx ⋮ T.
 Proof.
-  intros Hef Hvx. unfold tapp_tm.
-  eapply TT_Let with (L := dom Γ ∪ fv_value vx).
-  - exact Hef.
-  - intros x Hx.
-    change (<[x := Tx →ₜ T]> Γ ⊢ₑ
-      tapp (vfvar x) (open_value 0 (vfvar x) vx) ⋮ T).
-    rewrite (open_rec_lc_value vx (typing_value_lc _ _ _ Hvx) 0 (vfvar x)).
-    eapply TT_App.
-    + eapply VT_FVar. rewrite lookup_insert.
-      destruct (decide (x = x)); [reflexivity | congruence].
-    + eapply basic_typing_weaken_insert_value; [set_solver | exact Hvx].
-Qed.
-
-Lemma reduction_tapp_tm_intro ef vf vx v :
-  lc_value vx →
-  ef →* tret vf →
-  tapp vf vx →* tret v →
-  tapp_tm ef vx →* tret v.
-Proof.
-  intros Hvx Hef Happ.
-  unfold tapp_tm.
-  eapply reduction_lete_intro.
-  - apply body_tapp_tm_body. exact Hvx.
-  - exact Hef.
-  - change (tapp vf (open_value 0 vf vx) →* tret v).
-    rewrite (open_rec_lc_value vx Hvx 0 vf).
-    exact Happ.
+  intros Hef Hvx. remember (Tx →ₜ T) as Tf eqn:HTf.
+  revert Tx T vx Hvx HTf.
+  induction Hef; intros Tx0 T0 vx Hvx HTf; subst; simpl.
+  - eapply TT_App; eauto.
+  - eapply TT_Let with (T1 := T1) (L := L ∪ fv_value vx ∪ dom Γ).
+    + exact Hef.
+    + intros x Hx.
+      change (<[x:=T1]> Γ ⊢ₑ open_tm 0 (vfvar x) (tapp_tm e2 vx) ⋮ T0).
+      rewrite open_tapp_tm_lc_arg by exact (typing_value_lc _ _ _ Hvx).
+      refine (H0 x _ Tx0 T0 vx _ _).
+      * set_solver.
+      * eapply basic_typing_weaken_insert_value; [set_solver | exact Hvx].
+      * reflexivity.
+  - discriminate.
+  - eapply TT_Let with (L := dom Γ ∪ fv_value vx).
+    + eapply TT_App; eauto.
+    + intros x Hx.
+      cbn.
+      rewrite (open_rec_lc_value vx (typing_value_lc _ _ _ Hvx) 0 (vfvar x)).
+      eapply TT_App.
+      * eapply VT_FVar. rewrite lookup_insert.
+        destruct (decide (x = x)); [reflexivity | congruence].
+      * eapply basic_typing_weaken_insert_value; [set_solver | exact Hvx].
+  - eapply TT_Let with (L := dom Γ ∪ fv_value vx).
+    + eapply TT_Match; eauto.
+    + intros x Hx.
+      cbn.
+      rewrite (open_rec_lc_value vx (typing_value_lc _ _ _ Hvx) 0 (vfvar x)).
+      eapply TT_App.
+      * eapply VT_FVar. rewrite lookup_insert.
+        destruct (decide (x = x)); [reflexivity | congruence].
+      * eapply basic_typing_weaken_insert_value; [set_solver | exact Hvx].
 Qed.
 
 Lemma lc_tchoice et ef :
